theories/lang/notation.v
@@ -23,10 +23,8 @@ Notation "'case:' e0 'of' el" := (Case e0%E el%E)
 Notation "'if:' e1 'then' e2 'else' e3" := (If e1%E e2%E e3%E)
   (at level 200, e1, e2, e3 at level 200) : expr_scope.
 Notation "()" := LitUnit : val_scope.
-Notation "! e" := (Read Na1Ord e%E)
-  (at level 9, right associativity) : expr_scope.
-Notation "!ˢᶜ e" := (Read ScOrd e%E)
-  (at level 9, right associativity) : expr_scope.
+Notation "! e" := (Read Na1Ord e%E) (at level 9, format "! e") : expr_scope.
+Notation "!ˢᶜ e" := (Read ScOrd e%E) (at level 9, format "!ˢᶜ e") : expr_scope.
 Notation "e1 + e2" := (BinOp PlusOp e1%E e2%E)
   (at level 50, left associativity) : expr_scope.
 Notation "e1 - e2" := (BinOp MinusOp e1%E e2%E)
