theories/typing/case.v
@@ -1,0 +1,125 @@
+From iris.proofmode Require Import tactics.
+From lrust.lang Require Import heap.
+From lrust.lifetime Require Import borrow frac_borrow.
+From lrust.typing Require Export uninit uniq_bor shr_bor own sum.
+From lrust.typing Require Import lft_contexts type_context programs.
+
+Section case.
+  Context `{typeG Σ}.
+
+  (* FIXME : the doc does not give [p +ₗ #(S (ty.(ty_size))) ◁ ...]. *)
+  Lemma type_case_own E L C T p n tyl el:
+    Forall2 (λ ty e,
+      typed_body E L C ((p +ₗ #0 ◁ own n (uninit 1)) :: (p +ₗ #1 ◁ own n ty) ::
+         (p +ₗ #(S (ty.(ty_size))) ◁
+            own n (uninit (list_max (map ty_size tyl) - ty_size ty))) :: T) e ∨
+      typed_body E L C ((p ◁ own n (sum tyl)) :: T) e) tyl el →
+    typed_body E L C ((p ◁ own n (sum tyl)) :: T) (case: !p of el).
+  Proof.
+    iIntros (Hel tid qE) "#HEAP #LFT Hna HE HL HC HT". wp_bind p.
+    rewrite tctx_interp_cons. iDestruct "HT" as "[Hp HT]".
+    iApply (wp_hasty with "Hp"). iIntros (v Hv) "Hp".
+    iDestruct "Hp" as (l) "[EQ [H↦ Hf]]". iDestruct "EQ" as %[=->].
+    iDestruct "H↦" as (vl) "[H↦ Hown]".
+    iDestruct "Hown" as (i vl' vl'') "(>% & >EQlen & Hown)". subst.
+    simpl ty_size. iDestruct "EQlen" as %[=EQlen]. rewrite -EQlen. simpl length.
+    rewrite -Nat.add_1_l app_length -!freeable_sz_split
+            heap_mapsto_vec_cons heap_mapsto_vec_app.
+    iDestruct "H↦" as "(H↦i & H↦vl' & H↦vl'')".
+    iDestruct "Hf" as "(Hfi & Hfvl' & Hfvl'')".
+    rewrite nth_lookup.
+    destruct (tyl !! i) as [ty|] eqn:EQty; last iDestruct "Hown" as ">[]".
+    edestruct @Forall2_lookup_l as (e & He & Hety); eauto.
+    wp_read. iApply wp_case; [lia|by rewrite Nat2Z.id|]. iNext.
+    destruct Hety as [Hety|Hety]; iApply (Hety with "HEAP LFT Hna HE HL HC");
+      rewrite !tctx_interp_cons !tctx_hasty_val' /= ?Hv //; iFrame "HT".
+    - iDestruct (ty.(ty_size_eq) with "Hown") as %<-.
+      iSplitL "H↦i Hfi"; last iSplitR "H↦vl'' Hfvl''".
+      + rewrite shift_loc_0. iExists _. iFrame. iSplit. done. iExists [ #i].
+        rewrite heap_mapsto_vec_singleton.
+        iFrame. iExists [_], []. auto.
+      + iExists _. iFrame. iSplit. done. iExists _. iFrame.
+      + rewrite -EQlen app_length minus_plus uninit_sz -(shift_loc_assoc_nat _ 1).
+        iExists _. iFrame. iSplit. done. iExists _. iFrame. rewrite uninit_own. auto.
+    - iExists _. iSplit. done.
+      assert (EQf:=freeable_sz_split n 1). simpl in EQf. rewrite -EQf. clear EQf.
+      rewrite -EQlen app_length -freeable_sz_split. iFrame.
+      iExists (#i :: vl' ++ vl''). iNext.
+      rewrite heap_mapsto_vec_cons heap_mapsto_vec_app.
+      iFrame. iExists i, vl', vl''. rewrite /= app_length nth_lookup EQty. auto.
+  Qed.
+
+  Lemma type_case_uniq E L C T p κ tyl el:
+    lctx_lft_alive E L κ →
+    Forall2 (λ ty e,
+      typed_body E L C ((p +ₗ #1 ◁ &uniq{κ}ty) :: T) e ∨
+      typed_body E L C ((p ◁ &uniq{κ}sum tyl) :: T) e) tyl el →
+    typed_body E L C ((p ◁ &uniq{κ}sum tyl) :: T) (case: !p of el).
+  Proof.
+    iIntros (Halive Hel tid qE) "#HEAP #LFT Hna HE HL HC HT". wp_bind p.
+    rewrite tctx_interp_cons. iDestruct "HT" as "[Hp HT]".
+    iApply (wp_hasty with "Hp"). iIntros (v Hv) "Hp".
+    iDestruct "Hp" as (l P) "[[EQ HP] Hb]". iDestruct "EQ" as %[=->].
+    iMod (bor_iff with "LFT HP Hb") as "Hb". done.
+    iMod (Halive with "HE HL") as (q) "[Htok Hclose]". done.
+    iMod (bor_acc_cons with "LFT Hb Htok") as "[H↦ Hclose']". done.
+    iDestruct "H↦" as (vl) "[H↦ Hown]".
+    iDestruct "Hown" as (i vl' vl'') "(>% & >EQlen & Hown)". subst.
+    iDestruct "EQlen" as %[=EQlen].
+    rewrite heap_mapsto_vec_cons heap_mapsto_vec_app nth_lookup.
+    iDestruct "H↦" as "(H↦i & H↦vl' & H↦vl'')".
+    destruct (tyl !! i) as [ty|] eqn:EQty; last iDestruct "Hown" as ">[]".
+    edestruct @Forall2_lookup_l as (e & He & Hety); eauto.
+    wp_read. iApply wp_case; [lia|by rewrite Nat2Z.id|]. iNext.
+    iDestruct (ty.(ty_size_eq) with "Hown") as %EQlenvl'.
+    destruct Hety as [Hety|Hety].
+    - iMod ("Hclose'" $! (shift_loc l 1 ↦∗: ty.(ty_own) tid)%I
+            with "[H↦vl' Hown] [H↦i H↦vl'']") as "[Hb Htok]".
+      { iExists vl'. iFrame. }
+      { iIntros "!>Hown". iDestruct "Hown" as (vl'2) "[H↦ Hown]".
+        iExists (#i::vl'2++vl''). iIntros "!>". iNext.
+        iDestruct (ty.(ty_size_eq) with "Hown") as %EQlenvl'2.
+        rewrite heap_mapsto_vec_cons heap_mapsto_vec_app EQlenvl' EQlenvl'2.
+        iFrame. iExists _, _, _. iSplit. by auto.
+        rewrite /= -EQlen !app_length EQlenvl' EQlenvl'2 nth_lookup EQty /=. auto. }
+      iMod ("Hclose" with "Htok") as "[HE HL]".
+      iApply (Hety with "HEAP LFT Hna HE HL HC").
+      rewrite !tctx_interp_cons !tctx_hasty_val' /= ?Hv //. iFrame "HT".
+      iExists _, _. iFrame. iSplit. done. iSplit; iIntros "!>!#$".
+    - iMod ("Hclose'" with "* [H↦i H↦vl' H↦vl'' Hown] []") as "[Hb Htok]";
+        [|by iIntros "!>$"|].
+      { iExists (#i::vl'++vl'').
+        rewrite heap_mapsto_vec_cons heap_mapsto_vec_app -EQlen. iFrame. iNext.
+        iExists i, vl', vl''. rewrite nth_lookup EQty. auto. }
+      iMod ("Hclose" with "Htok") as "[HE HL]".
+      iApply (Hety with "HEAP LFT Hna HE HL HC").
+      rewrite !tctx_interp_cons !tctx_hasty_val' /= ?Hv //. iFrame "HT".
+      iExists _, _. iFrame. iSplit. done. iSplit; iIntros "!>!#$".
+  Qed.
+
+  Lemma type_case_shr E L C T p κ tyl el:
+    lctx_lft_alive E L κ →
+    Forall2 (λ ty e,
+      typed_body E L C ((p +ₗ #1 ◁ &shr{κ}ty) :: T) e ∨
+      typed_body E L C ((p ◁ &shr{κ}sum tyl) :: T) e) tyl el →
+    typed_body E L C ((p ◁ &shr{κ}sum tyl) :: T) (case: !p of el).
+  Proof.
+    iIntros (Halive Hel tid qE) "#HEAP #LFT Hna HE HL HC HT". wp_bind p.
+    rewrite tctx_interp_cons. iDestruct "HT" as "[Hp HT]".
+    iApply (wp_hasty with "Hp"). iIntros (v Hv) "Hp".
+    iDestruct "Hp" as (l) "[EQ Hl]". iDestruct "EQ" as %[=->].
+    iDestruct "Hl" as (i) "[#Hb Hshr]".
+    iMod (Halive with "HE HL") as (q) "[Htok Hclose]". done.
+    iMod (frac_bor_acc with "LFT Hb Htok") as (q') "[[H↦i H↦vl''] Hclose']". done.
+    rewrite nth_lookup.
+    destruct (tyl !! i) as [ty|] eqn:EQty; last iDestruct "Hshr" as "[]".
+    edestruct @Forall2_lookup_l as (e & He & Hety); eauto.
+    wp_read. iApply wp_case; [lia|by rewrite Nat2Z.id|]. iNext.
+    iMod ("Hclose'" with "[$H↦i $H↦vl'']") as "Htok".
+    iMod ("Hclose" with "Htok") as "[HE HL]".
+    destruct Hety as [Hety|Hety]; iApply (Hety with "HEAP LFT Hna HE HL HC");
+      rewrite !tctx_interp_cons !tctx_hasty_val' /= ?Hv //; iFrame "HT".
+    - iExists _. auto.
+    - iExists _. iSplit. done. iExists i. rewrite nth_lookup EQty /=. auto.
+  Qed.
+End case.
